lowering/exprLoweringPropsScript.sml
@@ -1374,7 +1374,7 @@ QED
 Theorem ci_mono_store_multi_results[local]:
   ∀ buf_op results offset sa. ci_mono sa (SND (store_multi_results buf_op results offset sa))
 Proof
-  Induct_on `results` >- simp[store_multi_results_def, ci_mono_comp_return] >> rpt strip_tac >> once_rewrite_tac[store_multi_results_def] >> ho_match_mp_tac ci_mono_bind >> conj_tac >- (rpt strip_tac >> IF_CASES_TAC >> simp[ci_mono_comp_return, ci_mono_emit_op]) >> rpt strip_tac >> ho_match_mp_tac ci_mono_ignore_bind >> conj_tac >- simp[ci_mono_emit_void] >> rpt strip_tac >> simp[]
+  Induct_on `results` >- simp[store_multi_results_def, ci_mono_comp_return] >> rpt strip_tac >> once_rewrite_tac[store_multi_results_def] >> ho_match_mp_tac ci_mono_bind >> conj_tac >- simp[ci_mono_emit_op] >> rpt strip_tac >> ho_match_mp_tac ci_mono_ignore_bind >> conj_tac >- simp[ci_mono_emit_void] >> rpt strip_tac >> simp[]
 QED
 
 Theorem ci_mono_compile_store_byte_chunks[local]:
